The $a$ and $b$ recurrence coefficients are given, respectively, by \citep[Eq.~(145)]{Zotter2009PhD}
\begin{equation}\label{eq:A1_Navigation_Filters:Recurrence_Coefficient_a}
a_l^m =
\begin{cases}
  \displaystyle \sqrt{\frac{(l - |m| + 1) (l + |m| + 1)}{(2 l + 1) (2 l + 3)}} & \text{for}~l \geq 0~\text{and}~0 \leq |m| \leq l, \\
  0 & \text{otherwise,}
\end{cases}
\end{equation}
and \citep[Eq.~(146)]{Zotter2009PhD}
\begin{equation}\label{eq:A1_Navigation_Filters:Recurrence_Coefficient_b}
b_l^m =
\begin{cases}
  \displaystyle \sqrt{\frac{(l - m - 1) (l - m)}{(2 l - 1) (2 l + 1)}} & \text{for}~l \geq 0~\text{and}~0 \leq m \leq l, \\
  \displaystyle -\sqrt{\frac{(l - m - 1) (l - m)}{(2 l - 1) (2 l + 1)}} & \text{for}~l \geq 0~\text{and}~-l \leq m < 0, \\
  0 & \text{otherwise.}
\end{cases}
\end{equation}